Proved primitive chan_inv lemmas

theories/mutref.v
@@ -58,7 +58,7 @@ Definition srv : val :=
       end.
 (* LATER : implement CAS (equality/binop) *)
 
-(* Remove procedure call between a client and a server *)
+(* Remote procedure call between a client and a server *)
 Definition rpc : val :=
   λ: "r" "m",
     let: "d" := newch in
@@ -83,13 +83,81 @@ Definition refΣ : gFunctors := #[ghost_varΣ val].
 Global Instance subG_refΣ {Σ} : subG refΣ Σ → refG Σ.
 Proof. solve_inG. Qed.
 
+
+Notation chan := loc.
+
+Section inv.
+
+  Context `{!chanG Σ, !refG Σ}.
+  Notation iProp := (iProp Σ).
+
+  Definition is_chan (s : chan) (R : val -> iProp) : iProp :=
+    (∃ (Ms : gmultiset val), s ↦ Ms ∗ ([∗ mset] m ∈ Ms, R m)).
+
+  Definition chan_inv N (s : chan) (R : val -> iProp): iProp :=
+    inv N (is_chan s R).
+
+  Lemma recv_chan_inv N (s : chan) (R : val -> iProp):
+    chan_inv N s R -∗
+    {{{ True }}} recv #s {{{ m, RET m; R m }}}.
+  Proof.
+    iIntros "#Hr !# %Φ _ HΦ".
+    rewrite /recv.
+    wp_rec.
+    iLöb as "IH".
+    wp_bind (chan_lang.TryRecv _).
+    iInv "Hr" as (M) "[>Hs HM]" "Hclose".
+    wp_apply (wp_tryrecv with "Hs").
+    iIntros (new_v) "Hnew".
+    iDestruct "Hnew" as "[[%v (%Hnew & Hs & %Hv)] | (%Hnew & Hs)]";
+      subst.
+    - rewrite big_sepMS_delete; eauto.
+      iDestruct "HM" as "[HR HM]".
+      iMod ("Hclose" with "[Hs HM]").
+      { iNext. iExists _. iSplitL "Hs"; done. }
+      iModIntro. wp_pures. iModIntro. iApply "HΦ"; done.
+    - iMod ("Hclose" with "[Hs HM]").
+      { iNext. iExists _. iSplitL "Hs"; first done.
+        rewrite big_sepMS_empty; done. }
+      iModIntro.
+      wp_pures. iApply "IH"; done.
+  Qed.
+
+  Lemma send_chan_inv N (s : chan) (R : val -> iProp) (m : val):
+    chan_inv N s R -∗
+    {{{ R m }}} Send #s m {{{ RET #(); True }}}.
+  Proof.
+    iIntros "#Hr !# %Φ Hm HΦ".
+    iInv "Hr" as (M) "[>Hs HM]" "Hclose".
+    wp_apply (wp_send with "Hs").
+    iIntros "Hs".
+    iMod ("Hclose" with "[Hs HM Hm]").
+    { iNext. iExists _. iSplitL "Hs"; first done.
+      rewrite comm. rewrite big_sepMS_insert. iFrame. }
+    iModIntro. iApply "HΦ"; done.
+  Qed.
+
+  (* TODO: make [newch] a non-keyword notation *)
+  Lemma new_chan_inv N (R : val -> iProp):
+    {{{ True }}} NewCh {{{ (s : chan), RET #s; chan_inv N s R }}}.
+  Proof.
+    iIntros "%Φ _ HΦ".
+    iApply wp_fupd.
+    wp_apply wp_newch; first done.
+    iIntros (l) "Hl".
+    iMod (inv_alloc N _ (is_chan l R) with "[Hl]") as "#Hinv".
+    { iNext. iExists _. iFrame. rewrite big_sepMS_empty. done. }
+    iModIntro. iApply "HΦ". done.
+  Qed.
+
+End inv.
+
 Section proof.
 
   Context `{!chanG Σ, !refG Σ}.
   Notation iProp := (iProp Σ).
 
   Let N := nroot .@ "mutref".
-
   (* We define a "mapsto" operator for the channels. In this case, the
    mapsto will correspond to a channel in the threadpool which stores a log of
    messages and that returns [v] from a [chan_get] operation. *)
@@ -100,58 +168,40 @@ Section proof.
     | Some v => SOMEV v
     end.
 
-  Notation chan := loc.
-
-  Definition chan_inv (γ : gname) (s : chan) (R : val -> iProp): iProp :=
-    ∃ (Ms : gmultiset val),
-      (* server *)
-      s ↦ Ms ∗ ([∗ mset] m ∈ Ms, R m).
+  (* For a reference that is a server, the invariant also keeps track
+    of what is stored in reply channel *)
+  (* TODO: refactor with [chan_inv] *)
+  (* TODO: rename [w] to [req] *)
+  Definition reply_payload (γ : gname) (old_v : val) (w : option val) (reply : val) : iProp :=
+    (* There exists some reply channel that stores sent messages *)
+    ∃ new_v, ghost_var γ (1/2) new_v ∗
+      match w with
+      | Some v => ⌜new_v = v ∧ reply = #()⌝
+      | None => ⌜new_v = old_v ∧ reply = new_v⌝ end.
 
   (* All messsages sent to an rpc is a pair of [reply_channel] and whether
     or not it is a GET/SET message *)
-  Definition rpc_payload (γ : gname) (s : chan) (m : val): iProp :=
+  Definition request_payload (γ : gname) (m : val): iProp :=
     ∃ (w : option val) (r : chan) (old_v : val),
-      (⌜m = (#r, option_to_val w)%V⌝ ∗ ghost_var γ (1/2) old_v).
-
-  (* For a reference that is a server, the invariant also keeps track
-    of what is stored in reply channel *)
-  Definition reply_inv (γ : gname) (r : chan) (old_v : val) (w : option val): iProp :=
-    (* There exists some reply channel that stores sent messages *)
-    ∃ Mr, r ↦ Mr ∗
-            [∗ mset] msg_v ∈ Mr, ∃ new_v, ghost_var γ (1/2) new_v ∗
-                                  match w with
-                                  | Some v => ⌜new_v = v ∧ msg_v = #()⌝
-                                  | None => ⌜new_v = old_v ∧ msg_v = new_v⌝ end.
-  Definition srv_payload (γ : gname) (s : chan) (m : val): iProp :=
-    ∃ (w : option val) (r : chan) (old_v : val),
-      (⌜m = (#r, option_to_val w)%V ∧ match w with
-                                      | Some v => old_v = v
-                                      | None => True end⌝ ∗
-        ghost_var γ (1/2) old_v ∗ reply_inv γ r old_v w).
-
-  Definition rpc_inv (γ : gname) (s : chan) := (chan_inv γ s (rpc_payload γ s)).
-  Definition srv_inv (γ : gname) (s : chan) := (chan_inv γ s (srv_payload γ s)).
+      (⌜m = (#r, option_to_val w)%V⌝ ∗
+        chan_inv N r (reply_payload γ old_v w) ∗
+        ghost_var γ (1/2) old_v).
 
   (* "Client state" *)
   Definition ref_mapsto (γ : gname) (v : val) : iProp :=
     ghost_var γ (1/2) v.
 
-  Definition is_rpc (γ : gname) (l : chan) : iProp :=
-    inv N (rpc_inv γ l).
+  Definition is_ref (γ : gname) (l : chan) : iProp :=
+    chan_inv N l (request_payload γ).
 
-  Definition is_srv (γ : gname) (l : chan) : iProp :=
-    inv N (srv_inv γ l).
-
-  Global Instance is_ref_persistent γ l : Persistent (is_rpc γ l).
-  Proof. apply _. Qed.
-  Global Instance is_srv_persistent γ l : Persistent (is_srv γ l).
+  Global Instance is_ref_persistent γ l : Persistent (is_ref γ l).
   Proof. apply _. Qed.
 
   Global Instance ref_mapsto_timeless γ l: Timeless (ref_mapsto γ l).
   Proof. apply _. Qed.
 
   Lemma chan_get_spec (v : val) l γ:
-    is_rpc γ l -∗
+    is_ref γ l -∗
     {{{ ref_mapsto γ v }}} chan_get #l @ ⊤ {{{ RET v ; ref_mapsto γ v }}}.
   Proof.
     iIntros "#Hr !# %Φ Hv HΦ".
@@ -323,8 +373,8 @@ Section proof.
     }
   Qed.
 
-  Lemma chan_ref_spec (γ : gname) (v : val):
-    {{{ ref_mapsto γ v }}} chan_ref v {{{ l, RET LitV (LitLoc l); is_srv γ l }}}.
+  Lemma chan_ref_spec (v : val):
+    {{{ True }}} chan_ref v {{{ l γ, RET LitV (LitLoc l); is_ref γ l ∗ ref_mapsto γ v }}}.
   Proof.
     iIntros (Φ) "Hv HΦ".
     wp_lam.
